dyn.v
@@ -1,0 +1,90 @@
+Require Import Coq.Logic.Decidable.
+Require Import PeanoNat.
+Require Import Coq.Strings.String.
+Require Import Ascii.
+Require Import Bool.
+Require Import Nat.
+Require Import Lia.
+
+Require Import LIR.maps.
+
+Require Import LIR.lir.
+
+
+Fixpoint dyn (e : IRE) : IRE :=
+  match e with
+  | IRENil => IREBox TgNil IRENil
+  | IRENum n => IREBox TgInt (IRENum n)
+  | IREPlus e1 e2 => IREBox TgInt (IREPlus (IREUnbox TgInt (dyn e1))
+                                           (IREUnbox TgInt (dyn e2)))
+  | IRECnst => IREBox TgTbl IRECnst
+  | IREAddr a => IREBox TgTbl (IREAddr a)
+  | IREGet e1 e2 => IREGet (IREUnbox TgTbl (dyn e1))
+                           (IREUnbox TgInt (dyn e2))
+  | IRESet e1 e2 e3 => IRESet (IREUnbox TgTbl (dyn e1))
+                              (IREUnbox TgInt (dyn e2))
+                              (dyn e3)
+  | IREVar var => IREVar var
+  | IRELamb var t e => IRELamb var IRTStar (dyn e)
+  | IRELambApp e1 e2 => IRELambApp (dyn e1) (dyn e2)
+  | IREFun e => IREBox TgFun (IREFun (dyn e))
+  | IREFunApp e1 e2 => IREFunApp (IREUnbox TgFun (dyn e1)) (dyn e2)
+  | IREBox _ e => dyn e
+  | IREUnbox _ e => dyn e
+  end.
+
+
+Lemma dynIdempotent : forall e, dyn e = dyn (dyn e).
+Proof. induction e; simpl; congruence. Qed.
+  
+
+Fixpoint dynType (t : EType) : EType :=
+  match t with
+  | ETn _ => IRTStar
+  | ETLamb t1 t2 => ETLamb IRTStar (dynType t2)
+  end.
+
+
+Fixpoint dynGamma (Γ : IREnvironment) : IREnvironment :=
+  match Γ with
+  | MEmpty => MEmpty
+  | MCons var T Γ' => MCons var IRTStar (dynGamma Γ')
+  end.
+
+
+Lemma TP2TGammaIn : forall Γ var T,
+    In Γ var = Some T -> In (dynGamma Γ) var = Some IRTStar.
+Proof.
+  induction Γ; intros var T H; simpl in *.
+  - easy.
+  - destruct (string_dec var s); eauto.
+Qed.
+
+
+Theorem dynTyping : forall Γ e T,
+    Γ |= e : T -> dynGamma Γ |= (dyn e) : dynType T.
+Proof.
+  intros Γ e T Hty.
+  induction Hty; eauto using IRTyping,TP2TGammaIn.
+Qed.
+
+
+Lemma dynValue : forall e, Value e -> Value (dyn e).
+Proof.
+  intros e HV. induction HV; simpl; eauto using Value.
+Qed.
+
+
+
+Lemma mPlus1 : forall e2 m e m' e',
+    m / e -->* m' / e' ->  m / IREPlus e e2 -->* m' / IREPlus e' e2.
+Proof.
+  intros e2.
+  intros m e m' e' Hmt.
+  remember (Some e') as E' eqn:Heq.
+  generalize dependent e'.
+  induction Hmt; intros e1 Heq; inversion Heq; subst;
+  eauto using step,multistep.
+Qed.
+
+
